Update end-to-end tests to use sys_safe

platform/Safety.v
@@ -11,15 +11,40 @@ Section OpSem.
     -> Labels stn l2 = Some w
     -> l1 = l2.
 
+  Definition labelSys (l : LabelMap.key) (pre : assert) :=
+    l = ("sys", Global "abort")
+    /\ pre = Precondition abortS None.
+
+  Hypothesis impSys :
+    LabelMap.fold (fun l pre P => labelSys l pre /\ P) (Imports m) True.
+
+  Lemma preserve : forall (ls : list (LabelMap.key * assert)) Q,
+    fold_left (fun P p => labelSys (fst p) (snd p) /\ P) ls Q
+    -> Q.
+    induction ls; simpl in *; intuition.
+    apply IHls in H; tauto.
+  Qed.
+
+  Theorem impSys' : forall l pre, LabelMap.MapsTo l pre (Imports m)
+    -> labelSys l pre.
+    rewrite LabelMap.fold_1 in impSys; intros.
+    apply LabelMap.elements_1 in H.
+    generalize dependent True.
+    clear impSys; induction H; simpl in *; intuition.
+
+    hnf in H; simpl in H; intuition subst.
+    apply preserve in impSys; tauto.
+
+    eauto.
+  Qed.    
+
   Hypothesis agree : forall l pre bl, LabelMap.MapsTo l (pre, bl) (Blocks m)
     -> exists w, Labels stn l = Some w
       /\ prog w = Some bl.
 
   Hypothesis agreeImp : forall l pre, LabelMap.MapsTo l pre (Imports m)
     -> exists w, Labels stn l = Some w
-      /\ prog w = None
-      /\ l = ("sys", Global "abort")
-      /\ pre = Precondition abortS None.
+      /\ prog w = None.
 
   Hypothesis omitImp : forall l w,
     Labels stn ("sys", l) = Some w
@@ -57,24 +82,24 @@ Section OpSem.
     tauto.
   Qed.
 
-  Theorem safety : forall st l pre bl, LabelMap.MapsTo l (pre, bl) (Blocks m)
-    -> Labels stn l = Some (fst st)
+  Theorem safety : forall st mn g pre, LabelMap.MapsTo (mn, Global g) pre (Exports m)
+    -> Labels stn (mn, Global g) = Some (fst st)
     -> interp (specs0 m stn) (pre (stn, snd st))
     -> sys_safe stn prog st.
     intros; hnf; intros.
 
-    apply reachable_sys in H2; post.
+    apply (ExportsSound ok) in H; destruct H.
 
+    apply reachable_sys in H2; post.
     eapply safety'' in H3; eauto.
     post.
+
+    specialize (impSys' _ _ H4); intro.
+    hnf in H2; intuition subst.
     apply agreeImp in H4; post; subst.
     eauto.
     case_eq (step stn prog st'); intros; eauto; congruence.
     
-    intros.
-    apply agreeImp in H2.
-    post; eauto.
-
     eauto.
   Qed.
 End OpSem.
